Cslib/Computability/LambdaCalculus/LocallyNameless/Stlc/Basic.lean
@@ -1,0 +1,164 @@
+/-
+Copyright (c) 2025 Chris Henson. All rights reserved.
+Released under Apache 2.0 license as described in the file LICENSE.
+Authors: Chris Henson
+-/
+
+import Cslib.Computability.LambdaCalculus.LocallyNameless.Stlc.Context
+import Cslib.Computability.LambdaCalculus.LocallyNameless.Untyped.Properties
+
+/-! # λ-calculus
+
+The simply typed λ-calculus, with a locally nameless representation of syntax.
+
+## References
+
+* [A. Chargueraud, *The Locally Nameless Representation*][Chargueraud2012]
+* See also <https://www.cis.upenn.edu/~plclub/popl08-tutorial/code/>, from which
+  this is partially adapted
+
+-/
+
+universe u v
+
+variable {Var : Type u} {Base : Type v} [DecidableEq Var]
+
+namespace LambdaCalculus.LocallyNameless.Stlc
+
+/-- Types of the simply typed lambda calculus. -/
+inductive Ty (Base : Type v)
+  /-- A base type, from a typing context. -/
+  | base : Base → Ty Base
+  /-- A function type. -/
+  | arrow : Ty Base → Ty Base → Ty Base
+
+scoped infixr:70 " ⤳ " => Ty.arrow
+
+open Term Ty
+
+/-- An extrinsic typing derivation for locally nameless terms. -/
+@[aesop unsafe [constructors (rule_sets := [LambdaCalculus.LocallyNameless.ruleSet])]]
+inductive Typing : Context Var (Ty Base) → Term Var → Ty Base → Prop
+  /-- Free variables, from a context judgement. -/
+  | var : Γ✓ → ⟨x,σ⟩ ∈ Γ → Typing Γ (fvar x) σ
+  /-- Lambda abstraction. -/
+  | abs (L : Finset Var) : (∀ x ∉ L, Typing (⟨x,σ⟩ :: Γ) (t ^ fvar x) τ) → Typing Γ t.abs (σ ⤳ τ) 
+  /-- Function application. -/
+  | app : Typing Γ t (σ ⤳ τ) → Typing Γ t' σ → Typing Γ (app t t') τ
+
+scoped notation:50 Γ " ⊢ " t " ∶" τ:arg => Typing Γ t τ
+
+namespace Typing
+
+variable {Γ Δ Θ : Context Var (Ty Base)}
+
+omit [DecidableEq Var] in
+/-- Typing is preserved on permuting a context. -/
+theorem perm (ht : Γ ⊢ t ∶τ) (hperm : Γ.Perm Δ) : Δ ⊢ t ∶ τ := by 
+  revert Δ
+  induction ht <;> intros Δ p
+  case app => aesop
+  case var => 
+    have := @p.mem_iff
+    aesop
+  case abs ih => 
+    constructor
+    intros x mem
+    exact ih x mem (by aesop)
+
+/-- Weakening of a typing derivation with an appended context. -/
+lemma weaken_aux : 
+    Γ ++ Δ ⊢ t ∶ τ → (Γ ++ Θ ++ Δ)✓ → (Γ ++ Θ ++ Δ) ⊢ t ∶ τ := by
+  generalize eq : Γ ++ Δ = Γ_Δ
+  intros h
+  revert Γ Δ Θ
+  induction h <;> intros Γ Δ Θ eq ok_Γ_Θ_Δ
+  case var => aesop
+  case app => aesop
+  case abs σ Γ' τ t xs ext ih =>
+    apply Typing.abs (xs ∪ (Γ ++ Θ ++ Δ).dom)
+    intros x _
+    have h : ⟨x, σ⟩ :: Γ ++ Δ = ⟨x, σ⟩ :: Γ' := by aesop
+    refine @ih x (by aesop) _ _ Θ h ?_
+    simp only [HasWellFormed.wf]
+    aesop
+
+/-- Weakening of a typing derivation by an additional context. -/
+lemma weaken : Γ ⊢ t ∶ τ → (Γ ++ Δ)✓ → Γ ++ Δ ⊢ t ∶ τ := by
+  intros der ok
+  rw [←List.append_nil (Γ ++ Δ)] at *
+  exact weaken_aux (by simp_all) ok
+
+omit [DecidableEq Var] in
+/-- Typing derivations exist only for locally closed terms. -/
+lemma lc : Γ ⊢ t ∶ τ → t.LC := by
+  intros h
+  induction h <;> constructor
+  case abs ih => exact ih
+  all_goals aesop
+
+variable [HasFresh Var]
+
+open Term
+
+/-- Substitution for a context weakened by a single type between appended contexts. -/
+lemma subst_aux :
+    (Δ ++ ⟨x, σ⟩ :: Γ) ⊢ t ∶ τ →
+    Γ ⊢ s ∶ σ → 
+    (Δ ++ Γ) ⊢ (t [x := s]) ∶ τ := by
+  generalize  eq : Δ ++ ⟨x, σ⟩ :: Γ = Θ
+  intros h
+  revert Γ Δ
+  induction h <;> intros Γ Δ eq der
+  case app => aesop
+  case var x' τ ok mem => 
+    simp only [subst_fvar]
+    rw [←eq] at mem
+    rw [←eq] at ok
+    cases (Context.wf_perm (by aesop) ok : (⟨x, σ⟩ :: Δ ++ Γ)✓)
+    case cons ok_weak _ =>
+    observe perm : (Γ ++ Δ).Perm (Δ ++ Γ)
+    by_cases h : x = x' <;> simp only [h]
+    case neg => aesop
+    case pos nmem =>
+      subst h eq
+      have nmem_Γ : ∀ γ, ⟨x, γ⟩ ∉ Γ := by
+        intros γ _
+        exact nmem x (List.mem_keys.mpr ⟨γ, by aesop⟩) rfl
+      have nmem_Δ : ∀ γ, ⟨x, γ⟩ ∉ Δ := by
+        intros γ _
+        exact nmem x (List.mem_keys.mpr ⟨γ, by aesop⟩) rfl
+      have eq' : τ = σ := by
+        simp only [List.mem_append, List.mem_cons, Sigma.mk.injEq, heq_eq_eq] at mem
+        match mem with | _ => aesop
+      rw [eq']
+      refine (weaken der ?_).perm perm
+      exact Context.wf_perm (id (List.Perm.symm perm)) ok_weak
+  case abs σ Γ' t T2 xs ih' ih =>
+    apply Typing.abs (xs ∪ {x} ∪ (Δ ++ Γ).dom)
+    intros x _
+    rw [
+      subst_def, 
+      subst_open_var _ _ _ _ _ der.lc,
+      show ⟨x, σ⟩ :: (Δ ++ Γ) = (⟨x, σ⟩ :: Δ) ++ Γ by aesop
+      ]
+    apply ih 
+    all_goals aesop  
+
+/-- Substitution for a context weakened by a single type. -/
+lemma typing_subst_head : 
+    ⟨x, σ⟩ :: Γ ⊢ t ∶ τ  → Γ ⊢ s ∶ σ → Γ ⊢ (t [x := s]) ∶ τ := by
+  intros weak der
+  rw [←List.nil_append Γ]
+  exact subst_aux weak der
+
+/-- Typing preservation for opening. -/
+@[aesop safe forward (rule_sets := [LambdaCalculus.LocallyNameless.ruleSet])]
+theorem preservation_open {xs : Finset Var} :
+  (∀ x ∉ xs, ⟨x, σ⟩ :: Γ ⊢ m ^ fvar x ∶ τ) → 
+  Γ ⊢ n ∶ σ → Γ ⊢ m ^ n ∶ τ
+  := by
+  intros mem der
+  have ⟨fresh, free⟩ := fresh_exists (xs ∪ m.fv)
+  rw [subst_intro fresh n m (by aesop) der.lc]
+  exact typing_subst_head (mem fresh (by aesop)) der
