Cslib/Computability/LambdaCalculus/LocallyNameless/Stlc/Context.lean
@@ -1,0 +1,57 @@
+/-
+Copyright (c) 2025 Chris Henson. All rights reserved.
+Released under Apache 2.0 license as described in the file LICENSE.
+Authors: Chris Henson
+-/
+
+import Cslib.Computability.LambdaCalculus.LocallyNameless.Untyped.AesopRuleset
+import Cslib.Syntax.HasWellFormed
+import Mathlib.Data.Finset.Defs
+import Mathlib.Data.Finset.Dedup
+import Mathlib.Data.List.Sigma
+
+/-! # λ-calculus
+
+Contexts as pairs of free variables and types.
+
+-/
+
+universe u v
+
+variable {Var : Type u} {Ty : Type v} [DecidableEq Var]
+
+namespace LambdaCalculus.LocallyNameless.Stlc
+
+/-- A typing context is a list of free variables and corresponding types. -/
+abbrev Context (Var : Type u) (Ty : Type v) := List ((_ : Var) × Ty)
+
+namespace Context
+
+/-- The domain of a context is the finite set of free variables it uses. -/
+@[simp]
+def dom : Context Var Ty → Finset Var := List.toFinset ∘ List.keys
+
+/-- A well-formed context. -/
+abbrev Ok : Context Var Ty → Prop := List.NodupKeys
+
+instance : HasWellFormed (Context Var Ty) :=
+  ⟨Ok⟩
+
+variable {Γ Δ : Context Var Ty}
+
+/-- Context membership is preserved on permuting a context. -/
+theorem dom_perm_mem_iff (h : Γ.Perm Δ) {x : Var} : 
+    x ∈ Γ.dom ↔ x ∈ Δ.dom := by
+  induction h <;> aesop
+
+omit [DecidableEq Var] in
+/-- Context well-formedness is preserved on permuting a context. -/
+@[aesop safe forward (rule_sets := [LambdaCalculus.LocallyNameless.ruleSet])]
+theorem wf_perm (h : Γ.Perm Δ) : Γ✓ → Δ✓ := (List.perm_nodupKeys h).mp
+
+omit [DecidableEq Var] in
+@[aesop safe forward (rule_sets := [LambdaCalculus.LocallyNameless.ruleSet])]
+theorem wf_strengthen : (Δ ++ ⟨x, σ⟩ :: Γ)✓ → (Δ ++ Γ)✓ := by
+  intros ok
+  have sl : List.Sublist (Δ ++ Γ) (Δ ++ ⟨x, σ⟩ :: Γ) := by simp
+  exact List.NodupKeys.sublist sl ok
