Cslib/Computability/LambdaCalculus/LocallyNameless/Stlc/Safety.lean
@@ -1,0 +1,92 @@
+/-
+Copyright (c) 2025 Chris Henson. All rights reserved.
+Released under Apache 2.0 license as described in the file LICENSE.
+Authors: Chris Henson
+-/
+
+import Cslib.Computability.LambdaCalculus.LocallyNameless.Stlc.Basic
+import Cslib.Computability.LambdaCalculus.LocallyNameless.Untyped.Basic
+import Cslib.Computability.LambdaCalculus.LocallyNameless.Untyped.Properties
+import Cslib.Computability.LambdaCalculus.LocallyNameless.Untyped.FullBetaConfluence
+
+/-! # λ-calculus
+
+Type safety of the simply typed λ-calculus, with a locally nameless representation of syntax.
+Theorems in this file are namespaced by their respective reductions.
+
+## References
+
+* [A. Chargueraud, *The Locally Nameless Representation*][Chargueraud2012]
+* See also <https://www.cis.upenn.edu/~plclub/popl08-tutorial/code/>, from which
+  this is partially adapted
+
+-/
+
+universe u v
+
+namespace LambdaCalculus.LocallyNameless
+
+open Stlc Typing
+
+variable {Var : Type u} {Base : Type v} {R : Term Var → Term Var → Prop}
+
+def PreservesTyping (R : Term Var → Term Var → Prop) (Base : Type v) := 
+  ∀ {Γ t t'} {τ : Ty Base}, Γ ⊢ t ∶ τ → R t t' → Γ ⊢ t' ∶ τ
+
+/-- If a reduction preserves types, so does its reflexive transitive closure. -/
+@[aesop safe forward (rule_sets := [LambdaCalculus.LocallyNameless.ruleSet])]
+theorem redex_preservesTyping : 
+    PreservesTyping R Base → PreservesTyping (Relation.ReflTransGen R) Base := by
+  intros _ _ _ _ _ _ redex
+  induction redex <;> aesop
+
+open Relation in
+/-- Confluence preserves type preservation. -/
+theorem confluence_preservesTyping {τ : Ty Base} : 
+    Confluence R → PreservesTyping R Base → Γ ⊢ a ∶ τ → 
+    (ReflTransGen R) a b → (ReflTransGen R) a c →
+    ∃ d, (ReflTransGen R) b d ∧ (ReflTransGen R) c d ∧ Γ ⊢ d ∶ τ := by
+  intros con p der ab ac
+  have ⟨d, bd, cd⟩ := con ab ac
+  exact ⟨d, bd, cd, redex_preservesTyping p der (ab.trans bd)⟩
+ 
+variable [HasFresh Var] [DecidableEq Var] {Γ : Context Var (Ty Base)}
+
+namespace Term.FullBeta
+
+/-- Typing preservation for full beta reduction. -/
+@[aesop safe forward (rule_sets := [LambdaCalculus.LocallyNameless.ruleSet])]
+theorem preservation : Γ ⊢ t ∶ τ → (t ⭢βᶠt') → Γ ⊢ t' ∶ τ := by
+  intros der
+  revert t'
+  induction der <;> intros t' step <;> cases step
+  case' abs.abs xs _ _ _ xs' _=> apply Typing.abs (xs ∪ xs')
+  case' app.beta der_l _ _ => cases der_l
+  all_goals aesop
+
+omit [HasFresh Var] [DecidableEq Var] in
+/-- A typed term either full beta reduces or is a value. -/
+theorem progress {t : Term Var} {τ : Ty Base} (ht : [] ⊢ t ∶τ) : t.Value ∨ ∃ t', t ⭢βᶠ t' := by
+  generalize eq : [] = Γ at ht
+  induction ht
+  case var => aesop
+  case abs xs mem ih =>
+    left
+    constructor
+    apply Term.LC.abs xs
+    intros _ mem'
+    exact (mem _ mem').lc
+  case app Γ M σ τ N der_l der_r ih_l ih_r => 
+    simp only [eq, forall_const] at *
+    right
+    cases ih_l
+    -- if the lhs is a value, beta reduce the application
+    next val =>
+      cases val
+      next M M_abs_lc => exact ⟨M ^ N, FullBeta.beta M_abs_lc der_r.lc⟩
+    -- otherwise, propogate the step to the lhs of the application
+    next step =>
+      obtain ⟨M', stepM⟩ := step
+      exact ⟨M'.app N, FullBeta.appR der_r.lc stepM⟩ 
+
+end LambdaCalculus.LocallyNameless.Term.FullBeta
