Cslib/Computability/LambdaCalculus/LocallyNameless/Untyped/FullBeta.lean
@@ -4,8 +4,8 @@ Released under Apache 2.0 license as described in the file LICENSE.
 Authors: Chris Henson
 -/
 
-import Cslib.Computability.LambdaCalculus.Untyped.LocallyNameless.Basic
-import Cslib.Computability.LambdaCalculus.Untyped.LocallyNameless.Properties
+import Cslib.Computability.LambdaCalculus.LocallyNameless.Untyped.Basic
+import Cslib.Computability.LambdaCalculus.LocallyNameless.Untyped.Properties
 import Cslib.Semantics.ReductionSystem.Basic
 
 /-! # β-reduction for the λ-calculus
