Cslib/Computability/LambdaCalculus/LocallyNameless/Untyped/Properties.lean
@@ -4,7 +4,7 @@ Released under Apache 2.0 license as described in the file LICENSE.
 Authors: Chris Henson
 -/
 
-import Cslib.Computability.LambdaCalculus.Untyped.LocallyNameless.Basic
+import Cslib.Computability.LambdaCalculus.LocallyNameless.Untyped.Basic
 
 universe u
 
